finished system-f, allegedly

TypedAssembly/SystemF/Step.lean
@@ -1,149 +1,137 @@
-import «TypedAssembly».SystemF.TermNf
+import «TypedAssembly».SystemF.Term
 
-def RenNf {Δ₁ Δ₂} (Γ₁ : CtxNf Δ₁) (Γ₂ : CtxNf Δ₂) : Rent Δ₁ Δ₂ → Type := 
-  fun rt =>
-  ∀ {t : Δ₁ ⊢nf⋆ ⋆}, Γ₁ ∋nf t → Γ₂ ∋nf rent_nf rt t
-
-def lift_nf {Δ₁ Δ₂ Γ₁ Γ₂} {rt : Rent Δ₁ Δ₂} (r : RenNf Γ₁ Γ₂ rt) {t : Δ₁ ⊢nf⋆ ⋆} : 
-  RenNf (Γ₁ ,, t) (Γ₂ ,, rent_nf rt t) rt 
-  | _, .here => .here
-  | _, .there x => .there (r x)
-
-def tlift_nf {Δ₁ Δ₂ Γ₁ Γ₂} {rt : Rent Δ₁ Δ₂} (r : RenNf Γ₁ Γ₂ rt) : 
-  ∀ {k}, RenNf (Γ₁ ,,⋆ k) (Γ₂ ,,⋆ k) (liftt rt)
-  | _, _, .move x => by
-    apply conv_ni_nf
-    any_goals (exact (LookupNf.move (r x)))
-    simp [weakent_nf]
-    repeat rw [←rent_nf_comp]
-    congr
-
-def ren_nf {Δ₁ Δ₂ Γ₁ Γ₂} {rt : Rent Δ₁ Δ₂} (r : RenNf Γ₁ Γ₂ rt) :
-  {t : Δ₁ ⊢nf⋆ ⋆} → (Γ₁ ⊢nf t) → (Γ₂ ⊢nf rent_nf rt t)
-  | _, .int i => .int i
-  | _, .var x => .var (r x)
-
-  | _, .fix e => .fix (ren_nf (lift_nf (lift_nf r)) e)
-  | _, .app e₁ e₂ => .app (ren_nf r e₁) (ren_nf r e₂)
-
-  | _, .Λ e => .Λ (ren_nf (tlift_nf r) e) 
-  | _, .sub e t => by
-    apply conv_ent_nf 
-    any_goals (exact (TermNf.sub (ren_nf r e) (rent_nf rt t)))
-    rw [rent_subst_nf_one]
-  
-  | _, .prim e₁ p e₂ => .prim (ren_nf r e₁) p (ren_nf r e₂)
-  | _, .pair e₁ e₂ => .pair (ren_nf r e₁) (ren_nf r e₂)
-  | _, .fst e => .fst (ren_nf r e)
-  | _, .snd e => .snd (ren_nf r e)
-  | _, .if0 e₁ e₂ e₃ => .if0 (ren_nf r e₁) (ren_nf r e₂) (ren_nf r e₃)
-
-def weaken_nf {Δ Γ} {t₁ t₂ : Δ ⊢nf⋆ ⋆} (e : Γ ⊢nf t₁) : (Γ ,, t₂ ⊢nf t₁) := conv_ent_nf rent_nf_id (ren_nf (conv_ni_nf (Eq.symm rent_nf_id) ∘ .there) e)
-
-def tweaken_nf {Δ Γ} (t : Δ ⊢nf⋆ ⋆) {k} (e : Γ ⊢nf t) : Γ ,,⋆ k ⊢nf weakent_nf t :=
-  ren_nf .move e
-
-def SubsNf {Δ₁ Δ₂} (Γ₁ : CtxNf Δ₁) (Γ₂ : CtxNf Δ₂) (st : SubstNf Δ₁ Δ₂) : Type := 
-  {t : Δ₁ ⊢nf⋆ ⋆} → (Γ₁ ∋nf t) → (Γ₂ ⊢nf subst_nf st t)
-
-def lifts_nf {Δ₁ Δ₂ Γ₁ Γ₂} (st : SubstNf Δ₁ Δ₂) (s : SubsNf Γ₁ Γ₂ st) {t : Δ₁ ⊢nf⋆ ⋆} :
-  SubsNf (Γ₁ ,, t) (Γ₂ ,, subst_nf st t) st
-  | _, .here => .var .here
-  | _, .there x => weaken_nf (s x)
-
-def tlifts_nf {Δ₁ Δ₂ Γ₁ Γ₂} (st : SubstNf Δ₁ Δ₂) (s : SubsNf Γ₁ Γ₂ st) : SubsNf (Γ₁ ,,⋆ k) (Γ₂ ,,⋆ k) (liftst_nf st) 
-  | t, x => by
-    cases x
-    rename_i t x
-    exact (conv_ent_nf (weakent_subst_nf st t) (tweaken_nf _ (s x)))
-
-def subs_nf {Δ₁ Δ₂ Γ₁ Γ₂} (st : SubstNf Δ₁ Δ₂) (s : SubsNf Γ₁ Γ₂ st) 
-  {t : Δ₁ ⊢nf⋆ ⋆} : (Γ₁ ⊢nf t) → (Γ₂ ⊢nf subst_nf st t)
-  | .int i => .int i
-  | .var x => s x
-
-  | .fix e => .fix (subs_nf st (lifts_nf st (lifts_nf st s)) e)
-  | .app e₁ e₂ => .app (subs_nf st s e₁) (subs_nf st s e₂)
-
-  | .Λ e => by
-    apply TermNf.Λ
-    rename_i t'
-    exact (conv_ent_nf (subst_liftt_nf st t')
-              (subs_nf (liftst_nf st) (tlifts_nf st s) e))
-  | .sub e t => by
-    apply conv_ent_nf
-    any_goals (exact (TermNf.sub (subs_nf st s e) (subst_nf st t)))
-    rw [subst_subst_nf_one]
-    simp [reify]
-
-  | .prim e₁ p e₂ => .prim (subs_nf st s e₁) p (subs_nf st s e₂)
-  | .pair e₁ e₂ => .pair (subs_nf st s e₁) (subs_nf st s e₂)
-  | .fst e => .fst (subs_nf st s e)
-  | .snd e => .snd (subs_nf st s e)
-  | .if0 e₁ e₂ e₃ => .if0 (subs_nf st s e₁) (subs_nf st s e₂) (subs_nf st s e₃)
-
-def extend_nf {Δ₁ Δ₂ Γ₁ Γ₂} (st : SubstNf Δ₁ Δ₂) (s : SubsNf Γ₁ Γ₂ st) {t : Δ₁ ⊢nf⋆ ⋆} : (Γ₂ ⊢nf subst_nf st t) → SubsNf (Γ₁ ,, t) Γ₂ st 
-  | e, _, .here => e
-  | _, _, .there x => s x
-
-def subs_extend : ∀ {Δ Γ k} {t₁ : Δ ,⋆ k ⊢nf⋆ ⋆} {t₂ : Δ ⊢nf⋆ k} (x : Γ ,,⋆ k ∋nf t₁), Γ ⊢nf subst_nf (extendt_nf (.ne ∘ .var) t₂) t₁ := by
-  intros
-  rename_i x
-  cases x
-  rename_i x
-  exact (conv_ent_nf (weakent_subst_nf_one _ _) (.var x))
-
-
-def subs_nf_one {Δ Γ} {t₁ t₂ : Δ ⊢nf⋆ ⋆} : (Γ ,, t₂ ⊢nf t₁) → (Γ ⊢nf t₂) → (Γ ⊢nf t₁) := by
-  intro e₂ e₁
-  apply conv_ent_nf
-  any_goals (exact (subs_nf (.ne ∘ .var) 
-                    (extend_nf (.ne ∘ .var)
-                     (conv_ent_nf (Eq.symm (subst_nf_id _)) ∘ .var)
-                     (conv_ent_nf (Eq.symm (subst_nf_id t₂)) e₁))
-                    e₂))
-  rw [subst_nf_id]
-
-macro b:term:80 "[" a:term:80 "]nf" : term =>
-  `(subs_nf_one $b $a)
-
-def tsubs_nf_one {Δ Γ k} (t₁ : Δ ,⋆ k ⊢nf⋆ ⋆) (e : Γ ,,⋆ k ⊢nf t₁) (t₂ : Δ ⊢nf⋆ k) : Γ ⊢nf (t₁[t₂]nf⋆) := subs_nf (extendt_nf (.ne ∘ .var) t₂) subs_extend e
-
-macro b:term:80 "⋆[" a:term:80 "]nf" : term =>
-  `(tsubs_nf_one $b $a)
-
-
-inductive Value : {Δ : Ctxt} → {Γ : CtxNf Δ} → {t : Δ ⊢nf⋆ ⋆} → (Γ ⊢nf t) → Prop where
+inductive Value : {Δ : Ctxt} → {Γ : Ctx Δ} → {t : Δ ⊢⋆ ⋆} → (Γ ⊢ t) → Prop where
   | v_int : Value (.int i)
-  | v_fix : Value (TermNf.fix e)
+  | v_fix : Value (.fix e)
   | v_Λ  : Value e → Value (.Λ e)
   | v_pair : Value e₁ → Value e₂ → Value (.pair e₁ e₂)
 
-inductive Step {Δ} {Γ : CtxNf Δ} : (Γ ⊢nf t) → (Γ ⊢nf t) → Prop
-  | app_exec : Value a → Step (.app (.fix e) a) ((e[.fix sorry]nf)[a]nf)
-  | app_left : Step a a' → Step (.app a e₁) (.app a' e₂)
-  | app_right : Value a → Step b b' → Step (.app a b) (.app a b')
+inductive Step : {Δ : Ctxt} → {Γ : Ctx Δ} → {t : Δ ⊢⋆ ⋆} → (Γ ⊢ t) → (Γ ⊢ t) → Prop
+  | app_exec   : Value a → Step (.app (.fix e) a) (e.[weaken a].[.fix e])
+  | app_right  : Value a → Step b b' → Step (.app a b) (.app a b')
+  | app_left   : Step a a' → Step (.app a e) (.app a' e)
+  
+  | Λ_steps    : Step e e' → Step (.Λ e) (.Λ e')
+  | sub_exec   : Step (.sub (.Λ e) t) (e⋆[t])
 
   | prim_exec  : Step (.prim (.int n₁) p (.int n₂)) (.int (interp p n₁ n₂))
-  | prim_left  : Step a a' → Step (.prim a p b) (.prim a' p b)
   | prim_right : Step b b' → Step (.prim (.int n) p b) (.prim (.int n) p b')
+  | prim_left  : Step a a' → Step (.prim a p b) (.prim a' p b)
+  
+  | pair_left  : Step a a' → Step ⟪ (!a, !b) ⟫ ⟪ (!a', !b) ⟫
+  | pair_right : Value a → Step b b' → Step ⟪ (!a, !b) ⟫ ⟪ (!a, !b') ⟫
 
-  | fst_exec   : Step nf⟪ π₁(!e, !_) ⟫ e
+  | fst_exec   : Step ⟪ π₁(!e, !e') ⟫ e
   | fst_steps  : Step e e' →  Step (.fst e) (.fst e')
 
-  | snd_exec   : Step nf⟪ π₂(!_, !e) ⟫ e
+  | snd_exec   : Step ⟪ π₂(!e', !e) ⟫ e
   | snd_steps  : Step e e' →  Step (.snd e) (.snd e')
 
-  | if0_exec   : Step nf⟪ if0 0 then !b else !c end ⟫ b
-  | ifn0_exec  : n ≠ 0 → Step nf⟪ if0 !(.int n) then !b else !c end ⟫ c
-  | if_steps   : Step a a' → Step nf⟪ if0 !a then !b else !c end ⟫ nf⟪ if0 !a' then !b else !c end ⟫
+  | if0_exec   : Step ⟪ if0 0 then !b else !c end ⟫ b
+  | ifn0_exec  : n ≠ 0 → Step ⟪ if0 !(.int n) then !b else !c end ⟫ c
+  | if_steps   : Step a a' → Step ⟪ if0 !a then !b else !c end ⟫ ⟪ if0 !a' then !b else !c end ⟫
 
-inductive MultiStep {Δ} {Γ : CtxNf Δ} {t : Δ ⊢nf⋆ ⋆} : (Γ ⊢nf t) → (Γ ⊢nf t) → Prop 
+namespace Step 
+  infixr:90 " ==> " => Step
+end Step
+open Step
+
+inductive MultiStep {Δ} {Γ : Ctx Δ} {t : Δ ⊢⋆ ⋆} : (Γ ⊢ t) → (Γ ⊢ t) → Prop 
   | refl {a} : MultiStep a a
-  | step {a b c} : Step a b → MultiStep b c → MultiStep a c
+  | step {a b c} : a ==> b → MultiStep b c → MultiStep a c
 
-theorem «1+1 -->* 2» : MultiStep (Γ := ∅) nf⟪ if0 0 then 1 + 1 else 5 end ⟫ nf⟪ 2 ⟫ :=
-  by repeat constructor
+namespace MultiStep 
+  infixr:90 " ==>* " => MultiStep
+end MultiStep
+open MultiStep
 
-theorem «fact 6 -->⋆ 720» : MultiStep (Γ := ∅) nf⟪ !fact 6 ⟫ nf⟪ 720 ⟫ := by repeat constructor
+example : ⟪ if0 0 then 1 + 1 * 1 else 5 * 1 end ⟫ ==>* (⟪ 2 ⟫ : ∅ ⊢ .int) := by
+  repeat constructor
+
+example : ⟪ if0 1 then 1 + 1 * 1 else 5 * 1 end ⟫ ==>* (⟪ 5 ⟫ : ∅ ⊢ .int) := by
+  repeat constructor
+  · intros contra; contradiction
+  · repeat constructor
+
+example : ⟪ !fact 0 ⟫ ==>* ⟪ 1 ⟫ := by
+  unfold fact
+  apply MultiStep.step
+  · apply Step.app_exec
+    constructor
+  · apply MultiStep.step
+    · simp [subs_one, conv_ent, subs]
+      apply Step.if0_exec
+    · apply MultiStep.refl
+
+example : ⟪ !fact 3 ⟫ ==>* ⟪ 6 ⟫ := by
+  unfold fact
+  apply MultiStep.step
+  · apply Step.app_exec
+    constructor
+  · apply MultiStep.step
+    · simp [subs_one, conv_ent, subs, extend]
+      apply Step.ifn0_exec
+      intros contra; contradiction
+    · constructor
+      · constructor
+        apply Step.app_right
+        · constructor
+        · constructor
+      · apply MultiStep.step
+        · apply Step.prim_right
+          repeat constructor
+        · simp [subs_one, conv_ent, subs, extend]
+          apply MultiStep.step
+          · apply Step.prim_right
+            apply Step.ifn0_exec
+            intros contra; contradiction
+          · constructor
+            apply Step.prim_right
+            apply Step.prim_right
+            apply Step.app_right
+            · constructor
+            · constructor
+            · constructor
+              · apply Step.prim_right
+                apply Step.prim_right
+                apply Step.app_exec
+                constructor
+              · simp [subs_one, conv_ent, subs, extend]
+                constructor
+                apply Step.prim_right
+                · apply Step.prim_right
+                  apply Step.ifn0_exec
+                  intros contra; contradiction
+                · constructor
+                  apply Step.prim_right
+                  · apply Step.prim_right
+                    apply Step.prim_right
+                    apply Step.app_right
+                    constructor
+                    constructor
+                  · constructor
+                    · apply Step.prim_right
+                      apply Step.prim_right
+                      apply Step.prim_right
+                      apply Step.app_exec
+                      constructor
+                    · constructor
+                      apply Step.prim_right
+                      apply Step.prim_right
+                      apply Step.prim_right
+                      simp [subs_one, conv_ent, subs]
+                      apply Step.if0_exec
+                      repeat constructor <;> repeat constructor
+
+example : ⟪ !intid 6 ⟫ ==>* ⟪ 6 ⟫ := by
+  unfold intid
+  unfold freeid
+  constructor
+  · apply Step.app_left
+    apply Step.sub_exec
+  constructor 
+  · apply Step.app_exec
+    constructor
+  · simp [subs_one, conv_ent, subs]
+    constructor
 
