TypedAssembly/SystemF/Term.lean
@@ -1,36 +1,12 @@
 import «TypedAssembly».SystemF.Typ
 import «TypedAssembly».SystemF.Prim
-
-inductive Ctx : Ctxt → Type where
-  | nil       : Ctx Ø
-  | snoc_kind : Ctx Δ → ∀ j, Ctx (Δ ,⋆ j)
-  | snoc_typ  : Ctx Δ → Δ ⊢⋆ ⋆ → Ctx Δ
-
-namespace Ctx
-  infixl:50 " ,, " => Ctx.snoc_typ
-  infixl:50 " ,,⋆ " => Ctx.snoc_kind
-  notation "∅" => Ctx.nil
-end Ctx
-open Ctx
-
-inductive Lookup : Ctx Δ → Δ ⊢⋆ ⋆ → Type where
-  | here  {Γ : Ctx Δ} {t : Δ ⊢⋆ ⋆}     : Lookup (Γ ,, t) t
-  | there {Γ : Ctx Δ} {t₁ t₂ : Δ ⊢⋆ ⋆} : Lookup Γ t₁ → Lookup (Γ ,, t₂) t₁
-  | move  {Γ : Ctx Δ} {t : Δ ⊢⋆ ⋆} {k} : Lookup Γ t →
-                                         Lookup (Γ ,,⋆ k) (weakent t)
-deriving Repr
-
-namespace Lookup
-  infix:40 " ∋ " => Lookup
-end Lookup
-open Lookup
-
+import «TypedAssembly».SystemF.TermEnv
 
 inductive Term : {Δ : Ctxt} → Ctx Δ → Δ ⊢⋆ ⋆ → Type where
   | int  {Γ : Ctx Δ} : Int → Term Γ .int
   | var  {Γ : Ctx Δ} {t : Δ ⊢⋆ ⋆} : Γ ∋ t → Term Γ t
 
-  | fix  {Γ : Ctx Δ} {t₁ t₂ : Δ ⊢⋆ ⋆} : Term (Γ ,, t₁ ,, ⋆⟪ !t₁ → !t₂ ⟫) t₂ → Term Γ ⋆⟪ !t₁ → !t₂ ⟫
+  | fix  {Γ : Ctx Δ} {t₁ t₂ : Δ ⊢⋆ ⋆} : Term (Γ ,, ⋆⟪ !t₁ → !t₂ ⟫ ,, t₁ ) t₂ → Term Γ ⋆⟪ !t₁ → !t₂ ⟫
   | app  {Γ : Ctx Δ} {t₁ t₂ : Δ ⊢⋆ ⋆} : Term Γ ⋆⟪ !t₁ → !t₂ ⟫ → Term Γ t₁ → Term Γ t₂
 
   | Λ    {Γ : Ctx Δ} {k} {t : Δ ,⋆ k ⊢⋆ ⋆} : Term (Γ ,,⋆ k) t → Term Γ ⋆⟪ ∀. !t ⟫
@@ -94,31 +70,163 @@ namespace Term
     | `( ⟪ if0 ($e₁, $e₂, $e₃) ⟫ ) => `(Term.if0 ⟪ $e₁ ⟫ ⟪ $e₂ ⟫ ⟪ $e₃ ⟫ )
 
     | `( ⟪ ( $e ) ⟫ ) => `( ⟪ $e ⟫ ) 
+
+
 end Term
 open Term
 
-def fact :  ∅ ⊢ ⋆⟪ int → int ⟫ :=
-  Term.fix (.if0 (.var (.there .here))
-            (.int 1)
-            (.prim (.var (.there .here)) .times (.app (.var .here) (Term.prim (.var (.there .here)) .minus (.int 1)))))
+  def fact :  ∅ ⊢ ⋆⟪ int → int ⟫ :=
+  Term.fix (.if0 (.var .here)
+      (.int 1)
+      (.prim (.var .here) .times (.app (.var (.there .here)) (Term.prim (.var .here) .minus (.int 1)))))
 
-def fact' : ∅ ⊢ ⋆⟪ int → int ⟫ := 
-  ⟪ λ. if0 #1 then
+  def fact' : ∅ ⊢ ⋆⟪ int → int ⟫ := 
+  ⟪ λ. if0 #0 then
          1
        else
-         #1 * (#0 (#1 - 1))
+         #0 * (#1 (#0 - 1))
        end ⟫
 
-theorem fact_eq_fact' : fact = fact' := rfl
+  theorem fact_eq_fact' : fact = fact' := rfl
 
-def sixfact := ⟪ !fact 6 ⟫
+  def sixfact := ⟪ !fact 6 ⟫
 
-def freeid : (∅ ,,⋆ ⋆) ⊢ ⋆⟪ ♯0 → ♯0 ⟫ :=
-  ⟪ λ. #1 ⟫
+  def freeid : (∅ ,,⋆ ⋆) ⊢ ⋆⟪ ♯0 → ♯0 ⟫ :=
+  ⟪ λ. #0 ⟫
 
-def intid : ∅ ⊢ ⋆⟪ int → int ⟫ :=
+  def intid : ∅ ⊢ ⋆⟪ int → int ⟫ :=
   ⟪ (Λ. !freeid)[int] ⟫
 
 def conv_ent {Δ Γ} {t₁ t₂ : Δ ⊢⋆ ⋆} : t₁ = t₂ → (Γ ⊢ t₁) → Γ ⊢ t₂
   | rfl, a => a
 
+def Ren {Δ₁ Δ₂} (Γ₁ : Ctx Δ₁) (Γ₂ : Ctx Δ₂) : Renτ Δ₁ Δ₂ → Type := 
+  fun rt =>
+  ∀ {t : Δ₁ ⊢⋆ ⋆}, Γ₁ ∋ t → Γ₂ ∋ renτ rt t
+
+def lift {Δ₁ Δ₂ Γ₁ Γ₂} {rt : Renτ Δ₁ Δ₂} (r : Ren Γ₁ Γ₂ rt) {t : Δ₁ ⊢⋆ ⋆} : 
+  Ren (Γ₁ ,, t) (Γ₂ ,, renτ rt t) rt 
+  | _, .here => .here
+  | _, .there x => .there (r x)
+
+def τlift {Δ₁ Δ₂ Γ₁ Γ₂} {rt : Renτ Δ₁ Δ₂} (r : Ren Γ₁ Γ₂ rt) : 
+  ∀ {k}, Ren (Γ₁ ,,⋆ k) (Γ₂ ,,⋆ k) (liftτ rt)
+  | _, _, .move x => by
+    apply conv_ni
+    rotate_left 1
+    · exact (Lookup.move (r x))
+    · simp [weakenτ]
+      repeat rw [←renτ_comp]
+      congr
+
+
+def ren {Δ₁ Δ₂ Γ₁ Γ₂} {rt : Renτ Δ₁ Δ₂} (r : Ren Γ₁ Γ₂ rt) :
+  {t : Δ₁ ⊢⋆ ⋆} → (Γ₁ ⊢ t) → (Γ₂ ⊢ renτ rt t)
+  | _, .int i => .int i
+  | _, .var x => .var (r x)
+
+  | _, .fix e => .fix (ren (lift (lift r)) e)
+  | _, .app e₁ e₂ => .app (ren r e₁) (ren r e₂)
+
+  | _, .Λ e => .Λ (ren (τlift r) e) 
+  | _, .sub e t => by
+    apply conv_ent; rotate_left 1
+    · exact (Term.sub (ren r e) (renτ rt t))
+    . rw [renτ_subsτ_one]
+  
+  | _, .prim e₁ p e₂ => .prim (ren r e₁) p (ren r e₂)
+  | _, .pair e₁ e₂ => .pair (ren r e₁) (ren r e₂)
+  | _, .fst e => .fst (ren r e)
+  | _, .snd e => .snd (ren r e)
+  | _, .if0 e₁ e₂ e₃ => .if0 (ren r e₁) (ren r e₂) (ren r e₃)
+
+def weaken {Δ Γ} {t₁ t₂ : Δ ⊢⋆ ⋆} (e : Γ ⊢ t₁) : (Γ ,, t₂ ⊢ t₁) := by
+  apply conv_ent; rotate_left 1
+  · exact (ren (conv_ni (Eq.symm renτ_id) ∘ .there) e)
+  · apply renτ_id
+
+def tweaken {Δ Γ} (t : Δ ⊢⋆ ⋆) {k} (e : Γ ⊢ t) : Γ ,,⋆ k ⊢ weakenτ t :=
+  ren .move e
+
+def Subs {Δ₁ Δ₂} (Γ₁ : Ctx Δ₁) (Γ₂ : Ctx Δ₂) (st : Subsτ Δ₁ Δ₂) : Type := 
+  {t : Δ₁ ⊢⋆ ⋆} → (Γ₁ ∋ t) → (Γ₂ ⊢ subsτ st t)
+
+def lifts {Δ₁ Δ₂ Γ₁ Γ₂} (st : Subsτ Δ₁ Δ₂) (s : Subs Γ₁ Γ₂ st) {t : Δ₁ ⊢⋆ ⋆} : Subs (Γ₁ ,, t) (Γ₂ ,, subsτ st t) st
+  | _, .here => .var .here
+  | _, .there x => weaken (s x)
+
+def tlifts {Δ₁ Δ₂ Γ₁ Γ₂} (st : Subsτ Δ₁ Δ₂) (s : Subs Γ₁ Γ₂ st) : Subs (Γ₁ ,,⋆ k) (Γ₂ ,,⋆ k) (liftsτ st) 
+  | t, x => by
+    cases x
+    rename_i t x
+    apply conv_ent; rotate_left 1
+    · exact (tweaken _ (s x))
+    · simp [weakenτ]
+      rw [←renτ_subsτ]
+      rw [←subsτ_renτ]
+      congr
+
+def subs {Δ₁ Δ₂ Γ₁ Γ₂} (st : Subsτ Δ₁ Δ₂) (s : Subs Γ₁ Γ₂ st) 
+  {t : Δ₁ ⊢⋆ ⋆} : (Γ₁ ⊢ t) → (Γ₂ ⊢ subsτ st t)
+  | .int i => .int i
+  | .var x => s x
+
+  | .fix e => .fix (subs st (lifts st (lifts st s)) e)
+  | .app e₁ e₂ => .app (subs st s e₁) (subs st s e₂)
+
+  | .Λ e => by
+    apply Term.Λ
+    rename_i t'
+    apply conv_ent; rotate_left 1
+    · exact (subs (liftsτ st) (tlifts st s) e)
+    · congr
+  | .sub e t => by
+    apply conv_ent; rotate_left 1
+    · exact (Term.sub (subs st s e) (subsτ st t))
+    · rw [subsτ_subsτ_one] 
+
+  | .prim e₁ p e₂ => .prim (subs st s e₁) p (subs st s e₂)
+  | .pair e₁ e₂ => .pair (subs st s e₁) (subs st s e₂)
+  | .fst e => .fst (subs st s e)
+  | .snd e => .snd (subs st s e)
+  | .if0 e₁ e₂ e₃ => .if0 (subs st s e₁) (subs st s e₂) (subs st s e₃)
+
+def extend {Δ₁ Δ₂ Γ₁ Γ₂} (st : Subsτ Δ₁ Δ₂) (s : Subs Γ₁ Γ₂ st) {t : Δ₁ ⊢⋆ ⋆} : (Γ₂ ⊢ subsτ st t) → Subs (Γ₁ ,, t) Γ₂ st 
+  | e, _, .here => e
+  | _, _, .there x => s x
+
+def subs_extend {Δ Γ k} {t₁ : Δ ,⋆ k ⊢⋆ ⋆} {t₂ : Δ ⊢⋆ k} (x : Γ ,,⋆ k ∋ t₁): Γ ⊢ subsτ (extendτ .var t₂) t₁ := by
+  cases x
+  rename_i x
+  apply conv_ent; rotate_left 1
+  · exact (.var x)
+  · simp [weakenτ]
+    rw [←subsτ_renτ]
+    have : (fun {j} => extendτ (fun {j} => Typ.var) t₂ ∘ Lookupt.there) = fun {j} => @Typ.var Δ j := by
+      funext j x
+      cases x <;> rfl
+    rw [this, subsτ_id]
+
+def subs_one {Δ Γ} {t₁ t₂ : Δ ⊢⋆ ⋆} : (Γ ,, t₂ ⊢ t₁) → (Γ ⊢ t₂) → (Γ ⊢ t₁) := by
+  intro e₂ e₁
+  apply conv_ent; rotate_left 1
+  · exact (subs .var
+      (extend .var
+       (conv_ent (Eq.symm (subsτ_id _)) ∘ .var)
+       (conv_ent (Eq.symm (subsτ_id t₂)) e₁))
+      e₂)
+  · rw [subsτ_id]
+
+macro b:term:80 ".[" a:term:80 "]" : term =>
+  `(subs_one $b $a)
+
+def tsubs_one {Δ Γ k} {t₁ : Δ ,⋆ k ⊢⋆ ⋆} (e : Γ ,,⋆ k ⊢ t₁) (t₂ : Δ ⊢⋆ k) : Γ ⊢ (t₁[t₂]⋆) := subs (extendτ .var t₂) subs_extend e
+
+macro b:term:80 "⋆[" a:term:80 "]" : term =>
+  `(tsubs_one $b $a)
+
+example : (⟪ #0 ⟫.[⟪ (1, 2) ⟫] : ∅ ⊢ ⋆⟪ int × int ⟫) =
+           ⟪ (1, 2) ⟫                               := rfl
+
+example : (⟪ λ. #1 #0 ⟫.[⟪ (6, 9) ⟫] : ∅  ⊢ ⋆⟪ int → int ⟫) =
+           ⟪ λ. #1 #0 ⟫                                    := rfl
