TypedAssembly/SystemF/Kind.lean
@@ -1,9 +1,11 @@
+import «TypedAssembly»
 
+/-- We do not support higher Typs -/
 inductive Kind where
   | star
   deriving BEq, DecidableEq, Repr
 
 namespace Kind 
-  notation "⋆" => Kind.star
+  notation " ⋆ " => Kind.star
 end Kind
 open Kind
