TypedAssembly/SystemF/Prim.lean
@@ -4,6 +4,7 @@ inductive Prim where
   | times
   deriving Repr, BEq, DecidableEq
 
+@[reducible, simp]
 abbrev interp : Prim → (Int → Int → Int)
   | .plus => Int.add
   | .minus => Int.sub
