TypedAssembly/SystemF/TermEnv.lean
@@ -1,0 +1,29 @@
+import «TypedAssembly».SystemF.Typ
+
+inductive Ctx : Ctxt → Type where
+  | nil       : Ctx Ø
+  | snoc_kind : Ctx Δ → ∀ j, Ctx (Δ ,⋆ j)
+  | snoc_typ  : Ctx Δ → Δ ⊢⋆ ⋆ → Ctx Δ
+
+namespace Ctx
+  infixl:50 " ,, " => Ctx.snoc_typ
+  infixl:50 " ,,⋆ " => Ctx.snoc_kind
+  notation " ∅ " => Ctx.nil
+end Ctx
+open Ctx
+
+inductive Lookup : Ctx Δ → Δ ⊢⋆ ⋆ → Type where
+  | here  {Γ : Ctx Δ} {t : Δ ⊢⋆ ⋆}     : Lookup (Γ ,, t) t
+  | there {Γ : Ctx Δ} {t₁ t₂ : Δ ⊢⋆ ⋆} : Lookup Γ t₁ → Lookup (Γ ,, t₂) t₁
+  | move  {Γ : Ctx Δ} {t : Δ ⊢⋆ ⋆} {k} : Lookup Γ t →
+                                         Lookup (Γ ,,⋆ k) (weakenτ t)
+deriving Repr
+
+namespace Lookup
+  infix:40 " ∋ " => Lookup
+end Lookup
+open Lookup
+
+def conv_ni {Δ Γ} {t₁ t₂ : Δ ⊢⋆ ⋆} : t₁ = t₂ → (Γ ∋ t₁) → Γ ∋ t₂
+  | rfl, a => a
+
